src/Typing.v
@@ -1,13 +1,14 @@
-From TLC Require Import LibString LibLN.
-From MCore Require Import Syntax Tactics.
+From TLC Require Import LibString LibList LibSet LibMap.
+From MCore Require Import Syntax Ctx Tactics.
+Import LibListNotation.
 
 Module Typing (P : PAT).
-  Module S := Syntax P.
-  Export S.
+  Module C := Ctx P.
+  Export C.
 
   Module Type PATCHECK.
-    Parameter ok_pat : env -> pat -> type -> env -> Prop.
-    Parameter matches_contradictory : env -> Prop.
+    Parameter ok_pat : ctx -> pat -> type -> ctx -> Prop.
+    Parameter matches_contradictory : ctx -> Prop.
     Parameter pats_compatible : list pat -> type -> Prop.
     Parameter pats_exhaustive : list pat -> type -> Prop.
   End PATCHECK.
@@ -19,19 +20,18 @@ Module Typing (P : PAT).
     (** TYPING RELATION DEFINITIONS **)
     (*********************************)
 
-    Definition ok_data (Gamma : env) (d : data) : Prop :=
-      ok d /\
+    Definition ok_data (Gamma : ctx) (d : data) : Prop :=
       forall T cons,
-        binds T cons d ->
-        binds T BindTName Gamma /\
+        d[T] = cons ->
+        tname_in T Gamma /\
           forall K,
-            K \in cons -> exists d ty, binds K (BindCon d ty T) Gamma
+            K \in (cons : set con) -> exists d ty, con_in K d ty T Gamma
     .
 
-    Inductive ok_kind : env -> kind -> Prop :=
-    | TypeOk : forall {Gamma : env},
+    Inductive ok_kind : ctx -> kind -> Prop :=
+    | TypeOk : forall Gamma,
         ok_kind Gamma KiType
-    (* | DataOk : forall {Gamma : env} {d : data}, *)
+    (* | DataOk : forall {Gamma : ctx} {d : data}, *)
     (*     ok_data Gamma d -> *)
     (*     ok_kind Gamma (KiData d) *)
     .
@@ -39,77 +39,72 @@ Module Typing (P : PAT).
      Hint Constructors ok_kind : mcore.
 
     Reserved Notation "Gamma |= T ~:: k " (at level 50).
-    Inductive ok_type : env -> type -> kind -> Prop :=
+    Inductive ok_type : ctx -> type -> kind -> Prop :=
     | KVar : forall Gamma tv k,
-        ok_env Gamma ->
-        binds tv (BindTVar k) Gamma ->
+        ok_ctx Gamma ->
+        tvar_in tv k Gamma ->
         Gamma |= TyFVar tv ~:: k
     | KArr : forall Gamma ty1 ty2,
         Gamma |= ty1 ~:: KiType ->
         Gamma |= ty2 ~:: KiType ->
         Gamma |= TyArr ty1 ty2 ~:: KiType
-    | KAll : forall L Gamma k ty,
+    | KAll : forall Gamma k ty,
         ok_kind Gamma k ->
-        (forall X, X \notin L ->
-                   (Gamma & X ~ BindTVar k) |= {0 ~> TyFVar X} ty ~:: KiType) ->
+        Gamma & BindTVar k |= {0 ~> TyFVar (length Gamma)} ty ~:: KiType ->
         Gamma |= TyAll k ty ~:: KiType
-    (* | TyProd' : forall {Gamma : env} {ty1 ty2 : type}, *)
+    (* | TyProd' : forall {Gamma : ctx} {ty1 ty2 : type}, *)
     (*     ok_type Gamma ty1 KiType -> *)
     (*     ok_type Gamma ty2 KiType -> *)
     (*     ok_type Gamma (TyProd ty1 ty2) KiType *)
-    (* | TyCon' : forall {Gamma : env} {ty : type} {d : data} {T : tname}, *)
+    (* | TyCon' : forall {Gamma : ctx} {ty : type} {d : data} {T : tname}, *)
     (*     ok_type Gamma ty (KiData d) -> *)
     (*     T \indom d -> *)
     (*     ok_type Gamma (TyCon ty T) KiType *)
-    (* | TySem' : forall {Gamma : env} {ty1 ty2 : type} {ps : list pat}, *)
+    (* | TySem' : forall {Gamma : ctx} {ty1 ty2 : type} {ps : list pat}, *)
     (*     ok_type Gamma ty1 KiType -> *)
     (*     ok_type Gamma ty2 KiType -> *)
     (*     ok_type Gamma (TySem ty1 ty2 ps) KiType *)
-    (* | TyData' : forall {Gamma : env} {d : data}, *)
+    (* | TyData' : forall {Gamma : ctx} {d : data}, *)
     (*     ok_data Gamma d -> *)
     (*     ok_type Gamma (TyData d) (KiData d) *)
-    (* | TyDataSub' : forall {Gamma : env} {ty : type} {d1 d2 : data}, *)
+    (* | TyDataSub' : forall {Gamma : ctx} {ty : type} {d1 d2 : data}, *)
     (*     ok_type Gamma ty (KiData d1) -> *)
     (*     d2 \c d1 -> *)
     (*     (forall {T : tname}, d2[T] \c d1[T]) -> *)
     (*     ok_type Gamma ty (KiData d2) *)
     where " Gamma |= T ~:: k " := (ok_type Gamma T k)
 
-    with ok_env : env -> Prop :=
-    | EnvEmpty : ok_env empty
-    | EnvTName : forall Gamma X, ok_env Gamma -> X # Gamma -> ok_env (Gamma & X ~ BindTName)
-    | EnvCon   :
-      forall Gamma K d ty T,
-        ok_env Gamma ->
-        K # Gamma ->
+    with ok_ctx : ctx -> Prop :=
+    | CtxEmpty : ok_ctx empty
+    | CtxTName : forall Gamma, ok_ctx Gamma -> ok_ctx (Gamma & BindTName)
+    | CtxCon   :
+      forall Gamma d ty T,
+        ok_ctx Gamma ->
         ok_data Gamma d ->
         Gamma |= ty ~:: KiType ->
-        binds T BindTName Gamma ->
-        ok_env (Gamma & K ~ BindCon d ty T)
-    | EnvTVar : forall Gamma X k,
-        ok_env Gamma ->
-        X # Gamma ->
+        tname_in T Gamma ->
+        ok_ctx (Gamma & BindCon d ty T)
+    | CtxTVar : forall Gamma k,
+        ok_ctx Gamma ->
         ok_kind Gamma k ->
-        ok_env (Gamma & X ~ BindTVar k)
-    | EnvVar : forall Gamma x ty,
-        ok_env Gamma ->
-        x # Gamma ->
+        ok_ctx (Gamma & BindTVar k)
+    | CtxVar : forall Gamma ty,
+        ok_ctx Gamma ->
         Gamma |= ty ~:: KiType ->
-        ok_env (Gamma & x ~ BindVar ty)
-    | EnvMatch : forall Gamma M m,
-        ok_env Gamma ->
-        M # Gamma ->
-        ok_env (Gamma & M ~ BindMatch m)
+        ok_ctx (Gamma & BindVar ty)
+    | CtxMatch : forall Gamma m,
+        ok_ctx Gamma ->
+        ok_ctx (Gamma & BindMatch m)
     .
     #[export]
      Hint Constructors ok_type : mcore.
     #[export]
-     Hint Constructors ok_env : mcore.
+     Hint Constructors ok_ctx : mcore.
 
     Reserved Notation "Gamma |= t ~: T " (at level 50).
-    Inductive ok_term : env -> term -> type -> Prop :=
+    Inductive ok_term : ctx -> term -> type -> Prop :=
     | TVar : forall Gamma x ty,
-        ok_env Gamma ->
+        ok_ctx Gamma ->
         binds x (BindVar ty) Gamma ->
         Gamma |= TmFVar x ~: ty
     | TLam : forall L Gamma ty1 ty2 t,
@@ -130,27 +125,27 @@ Module Typing (P : PAT).
         Gamma |= t ~: TyAll k ty1 ->
         Gamma |= ty2 ~:: k ->
         Gamma |= TmTyApp t ty2 ~: ({0 ~> ty2}ty1)
-    (* | TmFix' : forall {Gamma : env} {ty : type} {t : term}, *)
+    (* | TmFix' : forall {Gamma : ctx} {ty : type} {t : term}, *)
     (*     ok_term Gamma t (TyArr ty ty) -> *)
     (*     ok_term Gamma (TmFix t) ty *)
-    (* | TmProd' : forall {Gamma : env} {ty1 ty2 : type} {t1 t2 : term}, *)
+    (* | TmProd' : forall {Gamma : ctx} {ty1 ty2 : type} {t1 t2 : term}, *)
     (*     ok_term Gamma t1 ty1 -> *)
     (*     ok_term Gamma t2 ty2 -> *)
     (*     ok_term Gamma (TmProd t1 t2) (TyProd ty1 ty2) *)
-    (* | TmProj1' : forall {Gamma : env} {ty1 ty2 : type} {t : term}, *)
+    (* | TmProj1' : forall {Gamma : ctx} {ty1 ty2 : type} {t : term}, *)
     (*     ok_term Gamma t (TyProd ty1 ty2) -> *)
     (*     ok_term Gamma (TmProj F1 t) ty1 *)
-    (* | TmProj2' : forall {Gamma : env} {ty1 ty2 : type} {t : term}, *)
+    (* | TmProj2' : forall {Gamma : ctx} {ty1 ty2 : type} {t : term}, *)
     (*     ok_term Gamma t (TyProd ty1 ty2) -> *)
     (*     ok_term Gamma (TmProj F2 t) ty2 *)
-    (* | TmCon' : forall {Gamma : env} {K : con} {d : data} *)
+    (* | TmCon' : forall {Gamma : ctx} {K : con} {d : data} *)
     (*                   {ty1 ty2 : type} {T : tname} {t : term}, *)
     (*     con_in K d ty1 T Gamma.(cons) -> *)
     (*     ok_type Gamma ty2 (KiData d) -> *)
     (*     ok_type Gamma ty2 (KiData (T \:= \{K})) -> *)
     (*     ok_term Gamma t (ty_subst ty1 ty2) -> *)
     (*     ok_term Gamma (TmCon K ty2 t) (TyCon ty2 T) *)
-    (* | TmMatch' : forall {Gamma : env} {vs : var_env} {t t1 t2 : term} *)
+    (* | TmMatch' : forall {Gamma : ctx} {vs : var_ctx} {t t1 t2 : term} *)
     (*                     {ty1 ty2 : type} {p : pat}, *)
     (*     ok_term Gamma t ty1 -> *)
     (*     ok_pat  Gamma p ty1 vs -> *)
@@ -159,13 +154,13 @@ Module Typing (P : PAT).
     (*     ok_term (Gamma <| matches ::= fun ms => NoMatch t p :: ms |>) *)
     (*             t2 ty2 -> *)
     (*     ok_term Gamma (TmMatch t p t1 t2) ty2 *)
-    (* | TmNever' : forall {Gamma : env} {ty : type}, *)
+    (* | TmNever' : forall {Gamma : ctx} {ty : type}, *)
     (*     matches_contradictory Gamma.(matches) -> *)
     (*     ok_term Gamma TmNever ty *)
-    (* | TmType' : forall {Gamma : env} {t : term} {ty : type}, *)
+    (* | TmType' : forall {Gamma : ctx} {t : term} {ty : type}, *)
     (*     ok_type Gamma ty KiType -> *)
     (*     ok_term (Gamma <| tnames ::= S |>) t ty *)
-    (* | TmConDef' : forall {Gamma : env} {d : data} *)
+    (* | TmConDef' : forall {Gamma : ctx} {d : data} *)
     (*                      {ty1 ty2 : type} {T : tname} *)
     (*                      {t : term}, *)
     (*     ok_data Gamma d -> *)
@@ -175,11 +170,11 @@ Module Typing (P : PAT).
     (*             t ty2 -> *)
     (*     ok_type Gamma ty2 KiType -> *)
     (*     ok_term Gamma (TmConDef d ty1 T t) ty2 *)
-    (* | TmSem' : forall {Gamma : env} {ty1 ty2 : type} *)
+    (* | TmSem' : forall {Gamma : ctx} {ty1 ty2 : type} *)
     (*                   {cases : list (pat * term)}, *)
     (*     ok_type Gamma ty1 KiType -> *)
     (*     Forall (fun (c : pat * term) => *)
-    (*               exists (vs : var_env), *)
+    (*               exists (vs : var_ctx), *)
     (*                 ok_pat Gamma (fst c) ty1 vs /\ *)
     (*                   ok_term (Gamma <| vars ::= fun vs' => vs ++ vs' |>) *)
     (*                           (snd c) ty2) *)
@@ -189,13 +184,13 @@ Module Typing (P : PAT).
     (*       Gamma *)
     (*       (TmSem ty1 cases) *)
     (*       (TySem ty1 ty2 (LibList.map fst cases)) *)
-    (* | TmComp' : forall {Gamma : env} {ty1 ty2 : type} *)
+    (* | TmComp' : forall {Gamma : ctx} {ty1 ty2 : type} *)
     (*                    {t1 t2 : term} {ps1 ps2 : list pat}, *)
     (*     ok_term Gamma t1 (TySem ty1 ty2 ps1) -> *)
     (*     ok_term Gamma t2 (TySem ty1 ty2 ps2) -> *)
     (*     pats_compatible (ps1 ++ ps2) ty1 -> *)
     (*     ok_term Gamma (TmComp t1 t2) (TySem ty1 ty2 (ps1 ++ ps2)) *)
-    (* | TmSemApp' : forall {Gamma : env} {ty1 ty2 : type} *)
+    (* | TmSemApp' : forall {Gamma : ctx} {ty1 ty2 : type} *)
     (*                      {t1 t2 : term} {ps : list pat}, *)
     (*     ok_term Gamma t1 (TySem ty1 ty2 ps) -> *)
     (*     ok_term Gamma t2 ty1 -> *)
@@ -210,13 +205,13 @@ Module Typing (P : PAT).
     (** PROPERTIES OF TYPING **)
     (**************************)
 
-    Lemma ok_env_ok :
+    Lemma ok_ctx_ok :
       forall Gamma,
-        ok_env Gamma ->
+        ok_ctx Gamma ->
         ok Gamma.
-    Proof. introv Henv ; induction* Henv. Qed.
+    Proof. introv Hctx ; induction* Hctx. Qed.
     #[export]
-     Hint Resolve ok_env_ok : mcore.
+     Hint Resolve ok_ctx_ok : mcore.
 
     Lemma ok_kind_weakening :
       forall G3 G1 G2 k,
@@ -227,10 +222,10 @@ Module Typing (P : PAT).
     Lemma ok_type_weakening :
       forall G3 G1 G2 T k,
         G1 & G3 |= T ~:: k ->
-        ok_env (G1 & G2 & G3) ->
+        ok_ctx (G1 & G2 & G3) ->
         G1 & G2 & G3 |= T ~:: k.
     Proof.
-      introv Hk Henv.
+      introv Hk Hctx.
       remember (G1 & G3) as Gamma. gen G3.
       induction* Hk; intros; substs.
       { Case "TyFVar". constructors*. apply* binds_weaken. }
@@ -239,16 +234,16 @@ Module Typing (P : PAT).
         constructor*. apply* ok_kind_weakening. }
     Qed.
 
-    Lemma ok_env_ok_type :
+    Lemma ok_ctx_ok_type :
       forall Gamma x T,
-        ok_env Gamma ->
+        ok_ctx Gamma ->
         binds x (BindVar T) Gamma ->
         Gamma |= T ~:: KiType.
     Proof.
-      introv Henv Hbind.
-      induction* Henv ; try (binds_cases Hbind ; apply_empty* ok_type_weakening).
-      { Case "EnvEmpty". false. apply* binds_empty_inv. }
-      { Case "EnvVar". inverts* EQ. }
+      introv Hctx Hbind.
+      induction* Hctx ; try (binds_cases Hbind ; apply_empty* ok_type_weakening).
+      { Case "CtxEmpty". false. apply* binds_empty_inv. }
+      { Case "CtxVar". inverts* EQ. }
     Qed.
 
     Lemma ok_type_lct :
@@ -263,7 +258,7 @@ Module Typing (P : PAT).
       forall Gamma t T,
         Gamma |= t ~: T ->
         lct T.
-    Proof with eauto using ok_env_ok_type, ok_type_lct.
+    Proof with eauto using ok_ctx_ok_type, ok_type_lct.
       introv hasType.
       induction* hasType...
       { Case "TmLam". constructors...
@@ -288,47 +283,47 @@ Module Typing (P : PAT).
     #[export]
      Hint Resolve ok_term_lc : mcore.
 
-    Lemma ok_env_push :
+    Lemma ok_ctx_push :
       forall G1 x b,
-        ok_env (G1 & x ~ b) ->
-        ok_env G1.
+        ok_ctx (G1 & x ~ b) ->
+        ok_ctx G1.
     Proof.
       introv Hwf.
       inverts Hwf ; try (apply eq_push_inv in H; inverts H as []; substs*).
       false. apply *empty_push_inv.
     Qed.
 
-    Lemma ok_type_ok_env :
+    Lemma ok_type_ok_ctx :
       forall Gamma T k,
         Gamma |= T ~:: k ->
-        ok_env Gamma.
+        ok_ctx Gamma.
     Proof.
       introv hasType.
       induction* hasType; pick_fresh_gen L x;
-        eauto using ok_env_push.
+        eauto using ok_ctx_push.
     Qed.
     #[export]
-     Hint Resolve ok_type_ok_env : mcore.
+     Hint Resolve ok_type_ok_ctx : mcore.
 
-    Lemma ok_term_ok_env :
+    Lemma ok_term_ok_ctx :
       forall Gamma t T,
         Gamma |= t ~: T ->
-        ok_env Gamma.
+        ok_ctx Gamma.
     Proof.
       introv hasType.
       induction* hasType; pick_fresh_gen L x;
-        eauto using ok_env_push.
+        eauto using ok_ctx_push.
     Qed.
     #[export]
-     Hint Resolve ok_term_ok_env : mcore.
+     Hint Resolve ok_term_ok_ctx : mcore.
 
     Lemma ok_term_weakening :
       forall G3 G2 G1 t T,
         G1 & G3 |= t ~: T ->
-        ok_env (G1 & G2 & G3) ->
+        ok_ctx (G1 & G2 & G3) ->
         G1 & G2 & G3 |= t ~: T.
     Proof.
-      introv hasType Henv. remember (G1 & G3) as H. gen G3.
+      introv hasType Hctx. remember (G1 & G3) as H. gen G3.
       induction hasType; intros; substs*.
       { Case "TmFVar". constructors*. apply* binds_weaken. }
       { Case "TmLam". apply_fresh* TLam as y.
@@ -365,7 +360,7 @@ Module Typing (P : PAT).
     Lemma ok_type_strengthening :
       forall G1 G2 x T1 T2 k,
         G1 & x ~ BindVar T2 & G2 |= T1 ~:: k ->
-        ok_env (G1 & G2) ->
+        ok_ctx (G1 & G2) ->
         G1 & G2 |= T1 ~:: k.
     Proof.
       introv Htk. remember (G1 & x ~ BindVar T2 & G2) as G. gen G2.
@@ -377,56 +372,56 @@ Module Typing (P : PAT).
         apply_ih_bind* H1. constructor*. apply* ok_kind_strengthening. }
     Qed.
 
-    Lemma ok_env_con_inv :
+    Lemma ok_ctx_con_inv :
       forall Gamma K d ty T,
-        ok_env (Gamma & K ~ BindCon d ty T) ->
+        ok_ctx (Gamma & K ~ BindCon d ty T) ->
         ok_data Gamma d /\ Gamma |= ty ~:: KiType /\ binds T BindTName Gamma.
     Proof.
-      introv Henv.
-      inverts Henv ; try (apply eq_push_inv in H as (? & ? & ?); substs* ; splits* ; fequals).
+      introv Hctx.
+      inverts Hctx ; try (apply eq_push_inv in H as (? & ? & ?); substs* ; splits* ; fequals).
       false. apply* empty_push_inv.
     Qed.
 
-    Lemma ok_env_tvar_inv :
+    Lemma ok_ctx_tvar_inv :
       forall Gamma X k,
-        ok_env (Gamma & X ~ BindTVar k) ->
+        ok_ctx (Gamma & X ~ BindTVar k) ->
         ok_kind Gamma k.
     Proof.
-      introv Henv.
-      inverts Henv ; try (apply eq_push_inv in H as (? & ? & ?); substs* ; fequals).
+      introv Hctx.
+      inverts Hctx ; try (apply eq_push_inv in H as (? & ? & ?); substs* ; fequals).
       false. apply* empty_push_inv.
     Qed.
 
-    Lemma ok_env_var_inv :
+    Lemma ok_ctx_var_inv :
       forall Gamma x T,
-        ok_env (Gamma & x ~ BindVar T) ->
+        ok_ctx (Gamma & x ~ BindVar T) ->
         Gamma |= T ~:: KiType.
     Proof.
-      introv Henv.
-      inverts Henv ; try (apply eq_push_inv in H as (? & ? & ?); substs* ; fequals).
+      introv Hctx.
+      inverts Hctx ; try (apply eq_push_inv in H as (? & ? & ?); substs* ; fequals).
       false. apply* empty_push_inv.
     Qed.
 
-    Lemma ok_env_strengthening :
+    Lemma ok_ctx_strengthening :
       forall G1 x T G3,
-        ok_env (G1 & x ~ BindVar T & G3) ->
-        ok_env (G1 & G3).
+        ok_ctx (G1 & x ~ BindVar T & G3) ->
+        ok_ctx (G1 & G3).
     Proof.
-      introv Henv. induction G3 using env_ind.
-      { Case "Empty". rewrite concat_empty_r in *. apply* ok_env_push. }
+      introv Hctx. induction G3 using ctx_ind.
+      { Case "Empty". rewrite concat_empty_r in *. apply* ok_ctx_push. }
       { Case "Push". rewrite concat_assoc in *.
-        specializes IHG3 (ok_env_push _ _ _ Henv).
-        lets [? Hdisj] : ok_push_inv (ok_env_ok _ Henv).
+        specializes IHG3 (ok_ctx_push _ _ _ Hctx).
+        lets [? Hdisj] : ok_push_inv (ok_ctx_ok _ Hctx).
         destruct v.
         { SCase "BindTName". constructor~. }
-        { SCase "BindCon". forwards [ Hd (Htk & HT)]: ok_env_con_inv Henv.
+        { SCase "BindCon". forwards [ Hd (Htk & HT)]: ok_ctx_con_inv Hctx.
           constructor~.
           - applys ok_data_strengthening Hd.
           - applys* ok_type_strengthening Htk.
           - binds_cases HT ; auto. }
-        { SCase "BindTVar". forwards Hk: ok_env_tvar_inv Henv.
+        { SCase "BindTVar". forwards Hk: ok_ctx_tvar_inv Hctx.
           constructor~. applys ok_kind_strengthening Hk. }
-        { SCase "BindVar". forwards Htk: ok_env_var_inv Henv.
+        { SCase "BindVar". forwards Htk: ok_ctx_var_inv Hctx.
           constructor~. applys* ok_type_strengthening Htk. }
         { SCase "BindMatch". constructor~. } }
     Qed.
@@ -436,7 +431,7 @@ Module Typing (P : PAT).
         G1 & x ~ BindVar T2 & G2 |= t1 ~: T1 ->
         G1 |= t2 ~: T2 ->
         G1 & G2 |= [x => t2]t1 ~: T1.
-    Proof with eauto using ok_term_lc, ok_env_strengthening, ok_type_strengthening with mcore.
+    Proof with eauto using ok_term_lc, ok_ctx_strengthening, ok_type_strengthening with mcore.
       introv hasType1 hasType2.
       remember (G1 & x ~ BindVar T2 & G2) as G. gen G2.
       induction hasType1; intros; simpls; substs...
@@ -497,14 +492,14 @@ Module Typing (P : PAT).
       forall G1 G2 X T1 T2 k k',
         G1 & X ~ BindTVar k' & G2 |= T1 ~:: k ->
         G1 |= T2 ~:: k' ->
-        ok_env (G1 & map (bsubst X T2) G2) ->
+        ok_ctx (G1 & map (bsubst X T2) G2) ->
         G1 & map (bsubst X T2) G2 |= {X => T2} T1 ~:: k.
     Proof with eauto with mcore.
-      introv Hkt1 Hkt2 Henv.
+      introv Hkt1 Hkt2 Hctx.
       remember (G1 & X ~ BindTVar k' & G2) as G. gen G2.
       induction Hkt1; intros; substs; simpls*.
       { Case "TyFVar". solve_var.
-        + binds_get H0. lets* [Hok ?] : ok_concat_inv (ok_env_ok _ Henv).
+        + binds_get H0. lets* [Hok ?] : ok_concat_inv (ok_ctx_ok _ Hctx).
           apply_empty* ok_type_weakening.
         + binds_cases H0...
           constructors*. apply binds_concat_right.
@@ -516,50 +511,50 @@ Module Typing (P : PAT).
         rewrite~ tsubst_topen_comm.
         replaces (G1 & map (bsubst X T2) G2 & y ~ BindTVar k)
           with (G1 & map (bsubst X T2) (G2 & y ~ BindTVar k))...
-        + autorewrite with rew_env_map rew_env_concat ; auto.
+        + autorewrite with rew_ctx_map rew_ctx_concat ; auto.
         + apply~ H1.
-          * autorewrite with rew_env_concat ; auto.
-          * autorewrite with rew_env_map rew_env_concat... }
+          * autorewrite with rew_ctx_concat ; auto.
+          * autorewrite with rew_ctx_map rew_ctx_concat... }
     Qed.
 
-    Lemma bsubst_ok_env :
+    Lemma bsubst_ok_ctx :
       forall G1 G2 X T2 k,
         G1 |= T2 ~:: k ->
-        ok_env (G1 & X ~ BindTVar k & G2) ->
-        ok_env (G1 & map (bsubst X T2) G2).
+        ok_ctx (G1 & X ~ BindTVar k & G2) ->
+        ok_ctx (G1 & map (bsubst X T2) G2).
     Proof.
-      introv Htk Henv.
-      induction G2 using env_ind.
-      { Case "Empty". autorewrite with rew_env_map rew_env_concat in *.
-        apply* ok_env_push. }
-      { Case "Push". autorewrite with rew_env_map rew_env_concat in *.
-        specializes IHG2 (ok_env_push _ _ _ Henv).
-        lets [? Hdisj] : ok_push_inv (ok_env_ok _ Henv).
+      introv Htk Hctx.
+      induction G2 using ctx_ind.
+      { Case "Empty". autorewrite with rew_ctx_map rew_ctx_concat in *.
+        apply* ok_ctx_push. }
+      { Case "Push". autorewrite with rew_ctx_map rew_ctx_concat in *.
+        specializes IHG2 (ok_ctx_push _ _ _ Hctx).
+        lets [? Hdisj] : ok_push_inv (ok_ctx_ok _ Hctx).
         destruct v.
         { SCase "BindTName". constructor~. }
-        { SCase "BindCon". forwards (Hd & Htk' & HT): ok_env_con_inv Henv.
+        { SCase "BindCon". forwards (Hd & Htk' & HT): ok_ctx_con_inv Hctx.
           constructor~.
           - applys ok_data_bsubst. apply* ok_data_tvar_strengthening.
           - applys* ok_type_tsubst Htk.
           - binds_cases HT ; auto.
             replaces BindTName with (bsubst X T2 BindTName) ; auto. }
-        { SCase "BindTVar". forwards Hk: ok_env_tvar_inv Henv.
+        { SCase "BindTVar". forwards Hk: ok_ctx_tvar_inv Hctx.
           constructor~. applys ok_kind_bsubst. apply* ok_kind_tvar_strengthening. }
-        { SCase "BindVar". forwards Htk': ok_env_var_inv Henv.
+        { SCase "BindVar". forwards Htk': ok_ctx_var_inv Hctx.
           constructor~. applys* ok_type_tsubst Htk'. }
         { SCase "BindMatch". constructor~. } }
     Qed.
 
-    Lemma ok_env_concat :
+    Lemma ok_ctx_concat :
       forall G1 G2,
-        ok_env (G1 & G2) ->
-        ok_env G1.
+        ok_ctx (G1 & G2) ->
+        ok_ctx G1.
     Proof with eauto.
-      introv Henv.
-      induction G2 using env_ind.
-      { Case "Empty". rew_env_concat in *... }
-      { Case "Push". apply IHG2. rew_env_concat in *.
-        apply* ok_env_push. }
+      introv Hctx.
+      induction G2 using ctx_ind.
+      { Case "Empty". rew_ctx_concat in *... }
+      { Case "Push". apply IHG2. rew_ctx_concat in *.
+        apply* ok_ctx_push. }
     Qed.
 
     Lemma ok_type_notin :
@@ -580,23 +575,23 @@ Module Typing (P : PAT).
         applys~ topen_notin Y. }
     Qed.
 
-    Lemma env_bsubst_fresh :
+    Lemma ctx_bsubst_fresh :
       forall Gamma X T2,
-        ok_env Gamma ->
+        ok_ctx Gamma ->
         X # Gamma ->
         Gamma = map (bsubst X T2) Gamma.
-    Proof with eauto using ok_env_push.
-      introv Henv Hfresh.
-      induction Gamma using env_ind.
+    Proof with eauto using ok_ctx_push.
+      introv Hctx Hfresh.
+      induction Gamma using ctx_ind.
       { Case "Empty". rewrite~ map_empty. }
-      { Case "Push". autorewrite with rew_env_map.
+      { Case "Push". autorewrite with rew_ctx_map.
         rewrite <- IHGamma...
         destruct~ v ; repeat fequals ; unfold bsubst ; rewrite* tsubst_fresh.
         { SCase "BindCon".
-          apply ok_env_con_inv in Henv as (? & Hkt & ?).
+          apply ok_ctx_con_inv in Hctx as (? & Hkt & ?).
           apply* ok_type_notin. }
         { SCase "BindVar".
-          apply ok_env_var_inv in Henv.
+          apply ok_ctx_var_inv in Hctx.
           apply* ok_type_notin. } }
     Qed.
 
@@ -605,22 +600,22 @@ Module Typing (P : PAT).
         G1 & X ~ BindTVar k & G2 |= t ~: T1 ->
         G1 |= T2 ~:: k ->
         G1 & map (bsubst X T2) G2 |= [{X => T2}]t ~: ({X => T2}T1).
-    Proof with eauto using ok_env_strengthening, bsubst_ok_env with mcore.
-      introv hasType Henv.
+    Proof with eauto using ok_ctx_strengthening, bsubst_ok_ctx with mcore.
+      introv hasType Hctx.
       remember (G1 & X ~ BindTVar k & G2) as G. gen G2.
       induction hasType; intros; simpls; substs...
       { Case "TmFVar".
         binds_cases H0 ; constructors ;
           replaces (BindVar ({X => T2} ty)) with (bsubst X T2 (BindVar ty))...
-        apply ok_env_concat in H.
+        apply ok_ctx_concat in H.
         assert (X # G1) by apply* ok_push_inv.
-        rewrite* (@env_bsubst_fresh G1 X T2). }
+        rewrite* (@ctx_bsubst_fresh G1 X T2). }
       { Case "TmLam". apply_fresh* TLam as x.
-        + apply* ok_type_tsubst. apply* bsubst_ok_env.
+        + apply* ok_type_tsubst. apply* bsubst_ok_ctx.
         + rewrite tsubst_t_open_comm.
           replaces (G1 & map (bsubst X T2) G2 & x ~ BindVar ({X => T2}ty1))
             with (G1 & map (bsubst X T2) (G2 & x ~ BindVar ty1)).
-          autorewrite with rew_env_map rew_env_concat ; auto.
+          autorewrite with rew_ctx_map rew_ctx_concat ; auto.
           apply~ H1. rewrite~ concat_assoc. }
       { Case "TmTyLam". apply_fresh* TTyLam.
         + apply ok_kind_bsubst. apply* ok_kind_tvar_strengthening.
